midstream ncase extension

theories/examples/syntax/syntax.sig
@@ -3,9 +3,10 @@ abs     : Tm -> (bind Tm in Tm) -> Tm
 app     : Tm -> Tm -> Tm
 zero    : Tm
 succ    : Tm -> Tm 
-nrec    : (bind Tm in Tm) -> Tm -> Tm -> Tm
+ncase   : Tm -> Tm -> (bind Tm in Tm) -> Tm
 tnat    : Tm
 tpi     : Tm -> (bind Tm in Tm) -> Tm
 tuniv   : Tm   
+fix_    : Tm -> Tm
 
 
